p256: wip: clean up Hacl.Impl.P256.Sign

code/ecdsap256/Hacl.Impl.P256.Sign.fst
@@ -1,20 +1,15 @@
 module Hacl.Impl.P256.Sign
 
+open FStar.Mul
 open FStar.HyperStack.All
 open FStar.HyperStack
 module ST = FStar.HyperStack.ST
 
-open FStar.Mul
-open FStar.Math.Lemmas
-
 open Lib.IntTypes
 open Lib.Buffer
-open Lib.ByteSequence
 
 open Hacl.Spec.P256.Bignum
 open Hacl.Impl.P256.Bignum
-open Hacl.Impl.P256.Core
-open Hacl.Impl.P256.Qinv
 open Hacl.Impl.P256.Scalar
 open Hacl.Impl.P256.Point
 open Hacl.Impl.P256.PointMul
@@ -23,60 +18,55 @@ open Spec.Hash.Definitions
 open Hacl.Hash.SHA2
 
 module S = Spec.P256
+module LSeq = Lib.Sequence
+module BSeq = Lib.ByteSequence
 
-#set-options "--z3rlimit 100 --ifuel 0 --fuel 0"
+module QI = Hacl.Impl.P256.Qinv
 
+#set-options "--z3rlimit 50 --ifuel 0 --fuel 0"
 
-inline_for_extraction noextract
-val ecdsa_signature_step12: alg:S.hash_alg_ecdsa
-  -> mLen: size_t {v mLen >= S.min_input_length alg}
-  -> m: lbuffer uint8 mLen -> result: felem -> Stack unit
-  (requires fun h -> live h m /\ live h result )
-  (ensures fun h0 _ h1 -> modifies (loc result) h0 h1 /\
-    (
-      assert_norm (pow2 32 < pow2 61);
-      assert_norm (pow2 32 < pow2 125);
-      let hashM = S.hash_ecdsa alg (v mLen) (as_seq h0 m) in
-      let cutHashM = Lib.Sequence.sub hashM 0 32 in
-      as_nat h1 result = nat_from_bytes_be cutHashM % S.order
-    )
-  )
+val msg_as_felem:
+    alg:S.hash_alg_ecdsa
+  -> msg_len:size_t{v msg_len >= S.min_input_length alg}
+  -> msg:lbuffer uint8 msg_len
+  -> res:felem ->
+  Stack unit
+  (requires fun h ->
+    live h msg /\ live h res /\ disjoint msg res)
+  (ensures fun h0 _ h1 -> modifies (loc res) h0 h1 /\
+    (let hashM = S.hash_ecdsa alg (v msg_len) (as_seq h0 msg) in
+    as_nat h1 res = BSeq.nat_from_bytes_be (LSeq.sub hashM 0 32) % S.order))
 
-let ecdsa_signature_step12 alg mLen m result =
-  assert_norm (pow2 32 < pow2 61);
-  assert_norm (pow2 32 < pow2 125);
-  push_frame();
-    let h0 = ST.get() in
-  let sz: FStar.UInt32.t = match alg with | S.NoHash -> mLen | S.Hash a ->  Hacl.Hash.Definitions.hash_len a in
+[@CInline]
+let msg_as_felem alg msg_len msg res =
+  push_frame ();
+
+  let sz: size_t =
+    match alg with
+    | S.NoHash -> 32ul
+    | S.Hash a -> Hacl.Hash.Definitions.hash_len a in
+
   let mHash = create sz (u8 0) in
 
   begin
   match alg with
-    | S.NoHash -> copy mHash m
+    | S.NoHash -> copy mHash (sub msg 0ul 32ul)
     | S.Hash a -> match a with
-      |SHA2_256 -> hash_256 m mLen mHash
-      |SHA2_384 -> hash_384 m mLen mHash
-      |SHA2_512 -> hash_512 m mLen mHash
+      | SHA2_256 -> hash_256 msg msg_len mHash
+      | SHA2_384 -> hash_384 msg msg_len mHash
+      | SHA2_512 -> hash_512 msg msg_len mHash
   end;
 
-  let cutHash = sub mHash (size 0) (size 32) in
-  bn_from_bytes_be4 cutHash result;
+  let mHash32 = sub mHash 0ul 32ul in
+  bn_from_bytes_be4 mHash32 res;
+  qmod_short res res;
+  pop_frame ()
 
-  let h1 = ST.get() in
-
-  qmod_short result result;
-
-  lemma_core_0 result h1;
-  uints_from_bytes_be_nat_lemma #U64 #_ #4 (as_seq h1 cutHash);
-
-  pop_frame()
-
-#push-options "--ifuel 1"
 
 inline_for_extraction
-val ecdsa_signature_step45: x: felem
-  -> k: lbuffer uint8 (size 32)
-  -> tempBuffer: lbuffer uint64 (size 100)
+val ecdsa_signature_step45: x:felem
+  -> k:lbuffer uint8 32ul
+  -> tempBuffer:lbuffer uint64 (size 100)
   -> Stack uint64
     (requires fun h ->
       live h x /\ live h k /\ live h tempBuffer /\
@@ -98,14 +88,12 @@ val ecdsa_signature_step45: x: felem
 let ecdsa_signature_step45 x k tempBuffer =
   push_frame();
     let result = create (size 12) (u64 0) in
-    let tempForNorm = sub tempBuffer (size 0) (size 88) in
     secretToPublicWithoutNorm result k tempBuffer;
     norm_jacob_point_x result x;
     qmod_short x x;
   pop_frame();
     bn_is_zero_mask4 x
 
-#pop-options
 
 val lemma_power_step6: kInv: nat -> Lemma
   (S.qinv (fromDomain_ kInv) == toDomain_ (S.pow kInv (S.order - 2)))
@@ -116,7 +104,7 @@ let lemma_power_step6 kInv =
 
   //power_distributivity (kInv * S.modp_inv2_prime (pow2 256) S.order) (S.order - 2) S.order;
   //power_distributivity_2 kInv (S.modp_inv2_prime (pow2 256) S.order % S.order) (S.order - 2);
-  lemma_mod_mul_distr_r (S.pow kInv (S.order - 2)) (S.pow (S.modp_inv2_prime (pow2 256) S.order) (S.order - 2)) S.order;
+  Math.Lemmas.lemma_mod_mul_distr_r (S.pow kInv (S.order - 2)) (S.pow (S.modp_inv2_prime (pow2 256) S.order) (S.order - 2)) S.order;
 
   //lemma_pow_mod_n_is_fpow S.order (pow2 256 % S.order) (S.order - 2);
 
@@ -125,7 +113,7 @@ let lemma_power_step6 kInv =
   //lemma_pow_mod_n_is_fpow S.order inverse2_256 (S.order - 2);
   assert_norm(S.exp #S.order inverse2_256 (S.order - 2) == pow2 256 % S.order);
 
-  lemma_mod_mul_distr_r (S.pow kInv (S.order - 2)) (pow2 256) S.order;
+  Math.Lemmas.lemma_mod_mul_distr_r (S.pow kInv (S.order - 2)) (pow2 256) S.order;
   lemmaToDomain (S.pow kInv (S.order - 2))
 
 
@@ -161,7 +149,7 @@ let ecdsa_signature_step6 result kFelem z r da =
     fromDomainImpl z zBuffer;
     qadd rda zBuffer zBuffer;
     copy kInv kFelem;
-    qinv kInv;
+    QI.qinv kInv;
     qmul zBuffer kInv result;
   pop_frame();
       let br0 = as_nat h0 z + as_nat h0 r * as_nat h0 da in
@@ -174,22 +162,22 @@ let ecdsa_signature_step6 result kFelem z r da =
       lemmaToDomain br1;
       assert_norm ((S.modp_inv2_prime (pow2 256) S.order * pow2 256) % S.order = 1);
 
-      lemma_mod_mul_distr_l (fromDomain_ br0 * S.modp_inv2_prime (pow2 256) S.order) (br1 * pow2 256 % S.order) S.order;
-      lemma_mod_mul_distr_r (fromDomain_ br0 * S.modp_inv2_prime (pow2 256) S.order) (br1 * pow2 256) S.order;
+      Math.Lemmas.lemma_mod_mul_distr_l (fromDomain_ br0 * S.modp_inv2_prime (pow2 256) S.order) (br1 * pow2 256 % S.order) S.order;
+      Math.Lemmas.lemma_mod_mul_distr_r (fromDomain_ br0 * S.modp_inv2_prime (pow2 256) S.order) (br1 * pow2 256) S.order;
 
       assert_by_tactic (fromDomain_ br0 * S.modp_inv2_prime (pow2 256) S.order * (br1 * pow2 256) == fromDomain_ br0 * S.modp_inv2_prime (pow2 256) S.order * br1 * pow2 256) canon;
       assert_by_tactic (fromDomain_ br0 * br1 * (S.modp_inv2_prime (pow2 256) S.order * pow2 256) == fromDomain_ br0 * S.modp_inv2_prime (pow2 256) S.order * br1 * pow2 256) canon;
 
-      lemma_mod_mul_distr_r (fromDomain_ br0 * br1) (S.modp_inv2_prime (pow2 256) S.order * pow2 256) S.order;
+      Math.Lemmas.lemma_mod_mul_distr_r (fromDomain_ br0 * br1) (S.modp_inv2_prime (pow2 256) S.order * pow2 256) S.order;
       lemmaToDomain ((fromDomain_ br0 * br1) % S.order);
       lemmaFromDomain br0;
 
-      lemma_mod_mul_distr_l (br0 * S.modp_inv2_prime (pow2 256) S.order) br1 S.order;
-      lemma_mod_mul_distr_l (br0 * S.modp_inv2_prime (pow2 256) S.order * br1) (pow2 256) S.order;
+      Math.Lemmas.lemma_mod_mul_distr_l (br0 * S.modp_inv2_prime (pow2 256) S.order) br1 S.order;
+      Math.Lemmas.lemma_mod_mul_distr_l (br0 * S.modp_inv2_prime (pow2 256) S.order * br1) (pow2 256) S.order;
 
       assert_by_tactic (br0 * S.modp_inv2_prime (pow2 256) S.order * br1 * pow2 256 = br0 * br1 * (S.modp_inv2_prime (pow2 256) S.order * pow2 256)) canon;
-      lemma_mod_mul_distr_r (br0 * br1) (S.modp_inv2_prime (pow2 256) S.order * pow2 256) S.order;
-      lemma_mod_mul_distr_r br0 br1 S.order
+      Math.Lemmas.lemma_mod_mul_distr_r (br0 * br1) (S.modp_inv2_prime (pow2 256) S.order * pow2 256) S.order;
+      Math.Lemmas.lemma_mod_mul_distr_r br0 br1 S.order
 
 #push-options "--ifuel 1"
 
@@ -209,7 +197,7 @@ val ecdsa_signature_core: alg: S.hash_alg_ecdsa
     disjoint r s /\
     as_nat h privKeyAsFelem < S.order /\
     as_nat h s == 0 /\
-    nat_from_bytes_be (as_seq h k) < S.order
+    BSeq.nat_from_bytes_be (as_seq h k) < S.order
   )
   (ensures fun h0 flag h1 ->
     modifies (loc r |+| loc s) h0 h1 /\
@@ -218,11 +206,11 @@ val ecdsa_signature_core: alg: S.hash_alg_ecdsa
       assert_norm (pow2 32 < pow2 125);
       let hashM = S.hash_ecdsa alg (v mLen) (as_seq h0 m) in
       let cutHashM = Lib.Sequence.sub hashM 0 32 in
-      let z =  nat_from_bytes_be cutHashM % S.order in
+      let z =  BSeq.nat_from_bytes_be cutHashM % S.order in
       let (rxN, ryN, rzN), _ = S.montgomery_ladder_spec (as_seq h0 k) ((0,0,0), S.base_point) in
       let (xN, _, _) = S.norm_jacob_point (rxN, ryN, rzN) in
 
-      let kFelem = nat_from_bytes_be (as_seq h0 k) in
+      let kFelem = BSeq.nat_from_bytes_be (as_seq h0 k) in
       as_nat h1 r == xN % S.order /\
       as_nat h1 s == (z + (as_nat h1 r) * as_nat h0 privKeyAsFelem) * S.pow kFelem (S.order - 2) % S.order /\
       (
@@ -242,10 +230,10 @@ let ecdsa_signature_core alg r s mLen m privKeyAsFelem k =
   let tempBuffer = create (size 100) (u64 0) in
   let kAsFelem = create (size 4) (u64 0) in
   bn_from_bytes_be4 k kAsFelem;
-  ecdsa_signature_step12 alg mLen m hashAsFelem;
+  msg_as_felem alg mLen m hashAsFelem;
   let h1 = ST.get() in
   lemma_core_0 kAsFelem h1;
-  uints_from_bytes_be_nat_lemma #U64 #_ #4 (as_seq h0 k);
+  BSeq.uints_from_bytes_be_nat_lemma #U64 #_ #4 (as_seq h0 k);
   let step5Flag = ecdsa_signature_step45 r k tempBuffer in
   assert_norm (pow2 32 < pow2 61);
   ecdsa_signature_step6 s kAsFelem hashAsFelem r privKeyAsFelem;
@@ -256,55 +244,44 @@ let ecdsa_signature_core alg r s mLen m privKeyAsFelem k =
 
 #pop-options
 
+
 inline_for_extraction noextract
-val ecdsa_signature: alg: S.hash_alg_ecdsa
-  -> result: lbuffer uint8 (size 64)
-  -> mLen: size_t {v mLen >= S.min_input_length alg}
-  -> m: lbuffer uint8 mLen
-  -> privKey: lbuffer uint8 (size 32)
-  -> k: lbuffer uint8 (size 32) ->
+val ecdsa_signature:
+    alg:S.hash_alg_ecdsa
+  -> signature:lbuffer uint8 64ul
+  -> msg_len:size_t{v msg_len >= S.min_input_length alg}
+  -> msg:lbuffer uint8 msg_len
+  -> private_key:lbuffer uint8 32ul
+  -> nonce:lbuffer uint8 32ul ->
   Stack bool
   (requires fun h ->
-    live h result /\ live h m /\ live h privKey /\ live h k /\
-    disjoint result m /\
-    disjoint result privKey /\
-    disjoint result k /\
-    nat_from_bytes_be (as_seq h privKey) < S.order /\
-    nat_from_bytes_be (as_seq h k) < S.order
-  )
-  (ensures fun h0 flag h1 -> modifies (loc result) h0 h1 /\
-    (let sgnt = S.ecdsa_signature_agile alg (uint_v mLen) (as_seq h0 m) (as_seq h0 privKey) (as_seq h0 k) in
-      (flag <==> Some? sgnt) /\ (flag ==> (as_seq h1 result == Some?.v sgnt))))
+    live h signature /\ live h msg /\ live h private_key /\ live h nonce /\
+    disjoint signature msg /\ disjoint signature private_key /\ disjoint signature nonce /\
 
+    0 < BSeq.nat_from_bytes_be (as_seq h private_key) /\
+    BSeq.nat_from_bytes_be (as_seq h private_key) < S.order /\
+    0 < BSeq.nat_from_bytes_be (as_seq h nonce) /\
+    BSeq.nat_from_bytes_be (as_seq h nonce) < S.order)
+  (ensures fun h0 flag h1 -> modifies (loc signature) h0 h1 /\
+    (let sgnt = S.ecdsa_signature_agile alg (v msg_len)
+      (as_seq h0 msg) (as_seq h0 private_key) (as_seq h0 nonce) in
+     (flag <==> Some? sgnt) /\ (flag ==> (as_seq h1 signature == Some?.v sgnt))))
 
-let ecdsa_signature alg result mLen m privKey k =
-  push_frame();
+let ecdsa_signature alg signature msg_len msg private_key nonce =
+  push_frame ();
   let h0 = ST.get() in
-  assert_norm (pow2 32 < pow2 61);
-  let privKeyAsFelem = create (size 4) (u64 0) in
-  let r = create (size 4) (u64 0) in
-  let s = create (size 4) (u64 0) in
-  let resultR = sub result (size 0) (size 32) in
-  let resultS = sub result (size 32) (size 32) in
-  bn_from_bytes_be4 privKey privKeyAsFelem;
+  let privKeyAsFelem = create_felem () in
+  bn_from_bytes_be4 private_key privKeyAsFelem;
 
-  let h1 = ST.get() in
-  lemma_core_0 privKeyAsFelem h1;
-  uints_from_bytes_be_nat_lemma #U64 #_ #4 (as_seq h1 privKey);
-  let flag = ecdsa_signature_core alg r s mLen m privKeyAsFelem k in
+  let r = create_felem () in
+  let s = create_felem () in
 
-  let h2 = ST.get() in
+  let flag = ecdsa_signature_core alg r s msg_len msg privKeyAsFelem nonce in
 
-  bn_to_bytes_be4 r resultR;
-  lemma_core_0 r h2;
-  lemma_nat_from_to_intseq_le_preserves_value 4 (as_seq h2 r);
+  let signature_r = sub signature 0ul 32ul in
+  let signature_s = sub signature 32ul 32ul in
+  bn_to_bytes_be4 r signature_r;
+  bn_to_bytes_be4 s signature_s;
 
-  bn_to_bytes_be4 s resultS;
-  let h3 = ST.get() in
-  lemma_core_0 s h2;
-  lemma_nat_from_to_intseq_le_preserves_value 4 (as_seq h2 s);
-
-  pop_frame();
-
-  let open Hacl.Impl.P256.RawCmp in
-  unsafe_bool_of_u64  flag
+  pop_frame ();
+  Hacl.Impl.P256.RawCmp.unsafe_bool_of_u64 flag
